Solving the homogeneous problem for k=-1...
Our problem is:
 x \frac{d^{2}}{d x^{2}} y{\left(x \right)} + \frac{d}{d x} y{\left(x \right)} = 0
Solution is:
C_{1} + C_{2} \log{\left(x \right)}

Solving the homogeneous problem for k=1...
Our problem is:
 2 B \mu_{0}^{2} x y{\left(x \right)} + x \frac{d^{2}}{d x^{2}} y{\left(x \right)} + \frac{d}{d x} y{\left(x \right)} = 0
Solution is:
C_{1} J_{0}\left(\sqrt{2} x \sqrt{B \mu_{0}^{2}}\right) + C_{2} Y_{0}\left(\sqrt{2} x \sqrt{B \mu_{0}^{2}}\right)

Solving the homogeneous problem for k=0...
Our problem is:
 B \mu_{0}^{2} x + x \frac{d^{2}}{d x^{2}} y{\left(x \right)} + \frac{d}{d x} y{\left(x \right)} = 0
Solution is:
- \frac{B \mu_{0}^{2} x^{2}}{4} + C_{1} + C_{2} \log{\left(x \right)}

Solving the homogeneous problem for k=1...
Our problem is:
 2 B \mu_{0}^{2} x y{\left(x \right)} + x \frac{d^{2}}{d x^{2}} y{\left(x \right)} + \frac{d}{d x} y{\left(x \right)} = 0
Solution is:
C_{1} J_{0}\left(\sqrt{2} x \sqrt{B \mu_{0}^{2}}\right) + C_{2} Y_{0}\left(\sqrt{2} x \sqrt{B \mu_{0}^{2}}\right)
